src/cddl/pulse/CDDL.Pulse.AST.Bundle.fst
@@ -1,0 +1,1 @@
+module CDDL.Pulse.AST.Bundle
