src/cddl/pulse/CDDL.Pulse.Bundle.ArrayGroup.fst
@@ -1,0 +1,196 @@
+module CDDL.Pulse.Bundle.ArrayGroup
+include CDDL.Pulse.Bundle.Base
+include CDDL.Pulse.Parse.ArrayGroup
+open Pulse.Lib.Pervasives
+open CBOR.Spec.API.Type
+open CBOR.Pulse.API.Base
+
+inline_for_extraction noextract [@@noextract_to "krml"]
+noeq
+type array_bundle
+  (#cbor_array_iterator_t: Type0)
+  (cbor_array_iterator_match: perm -> cbor_array_iterator_t -> list cbor -> slprop)
+= {
+  ab_typ: Ghost.erased (array_group None);
+  ab_spec_type: Type0;
+  ab_spec: Ghost.erased (ag_spec ab_typ ab_spec_type true);
+  ab_impl_type: Type0;
+  ab_rel: rel ab_impl_type ab_spec_type;
+  ab_parser: impl_zero_copy_array_group cbor_array_iterator_match ab_spec.ag_parser ab_rel;
+}
+
+inline_for_extraction [@@bundle_get_impl_type_attr]
+let get_array_bundle_impl_type
+  (#cbor_array_iterator_t: Type0)
+  (cbor_array_iterator_match: perm -> cbor_array_iterator_t -> list cbor -> slprop)
+  (b: array_bundle cbor_array_iterator_match)
+: Pure Type0
+  (requires True)
+  (ensures fun t -> t == b.ab_impl_type) // guard if the number of fields changes
+= match b with
+  | Mkarray_bundle _ _ _ ab_impl_type _ _ -> ab_impl_type
+
+inline_for_extraction noextract [@@noextract_to "krml"; bundle_get_impl_type_attr ]
+let bundle_array
+  (#ty: Type0)
+  (#vmatch: perm -> ty -> cbor -> slprop)
+  (#cbor_array_iterator_t: Type)
+  (#cbor_array_iterator_match: perm -> cbor_array_iterator_t -> list cbor -> slprop)
+  (cbor_array_iterator_start: array_iterator_start_t vmatch cbor_array_iterator_match)
+  (ab: array_bundle cbor_array_iterator_match)
+: Tot (bundle vmatch)
+= {
+  b_typ = _;
+  b_spec_type = _;
+  b_spec = spec_array_group ab.ab_spec;
+  b_impl_type = _;
+  b_rel = _;
+  b_parser = impl_zero_copy_array cbor_array_iterator_start ab.ab_parser;
+}
+
+inline_for_extraction noextract [@@noextract_to "krml"; bundle_get_impl_type_attr]
+let bundle_array_group_ext
+  (#cbor_array_iterator_t: Type)
+  (#cbor_array_iterator_match: perm -> cbor_array_iterator_t -> list cbor -> slprop)
+  (ab: array_bundle cbor_array_iterator_match)
+  (#g2: Ghost.erased (array_group None))
+  (sp2: Ghost.erased (ag_spec g2 ab.ab_spec_type true))
+  (sq: squash (
+    array_group_included g2 ab.ab_typ /\
+    (forall (x: list cbor) . array_group_parser_spec_refinement g2 x ==> (
+       (sp2.ag_parser x <: ab.ab_spec_type) == (ab.ab_spec.ag_parser x <: ab.ab_spec_type)
+    ))
+  ))
+= {
+  ab_typ = _;
+  ab_spec_type = _;
+  ab_spec = sp2;
+  ab_impl_type = _;
+  ab_rel = _;
+  ab_parser = impl_zero_copy_array_group_ext ab.ab_parser sp2.ag_parser ();
+}
+
+inline_for_extraction noextract [@@noextract_to "krml"; bundle_get_impl_type_attr]
+let bundle_array_group_item
+  (#ty: Type0)
+  (#vmatch: perm -> ty -> cbor -> slprop)
+  (#cbor_array_iterator_t: Type)
+  (#cbor_array_iterator_match: perm -> cbor_array_iterator_t -> list cbor -> slprop)
+  (cbor_array_iterator_next: array_iterator_next_t vmatch cbor_array_iterator_match)
+  (b: bundle vmatch)
+: Tot (array_bundle cbor_array_iterator_match)
+= {
+  ab_typ = _;
+  ab_spec_type = _;
+  ab_spec = ag_spec_item b.b_spec;
+  ab_impl_type = _;
+  ab_rel = _;
+  ab_parser = impl_zero_copy_array_group_item cbor_array_iterator_next b.b_parser;
+}
+
+inline_for_extraction noextract [@@noextract_to "krml"; bundle_get_impl_type_attr]
+let bundle_array_group_concat
+  (#cbor_array_iterator_t: Type)
+  (#cbor_array_iterator_match: perm -> cbor_array_iterator_t -> list cbor -> slprop)
+  (length: array_iterator_length_t cbor_array_iterator_match)
+  (share: share_t cbor_array_iterator_match)
+  (gather: gather_t cbor_array_iterator_match)
+  (truncate: array_iterator_truncate_t cbor_array_iterator_match)
+  (b1: array_bundle cbor_array_iterator_match)
+  (v1: impl_array_group cbor_array_iterator_match b1.ab_typ)
+  (b2: array_bundle cbor_array_iterator_match)
+  (sq: squash (
+    array_group_concat_unique_weak b1.ab_typ b2.ab_typ
+  ))
+: Tot (array_bundle cbor_array_iterator_match)
+= {
+  ab_typ = _;
+  ab_spec_type = _;
+  ab_spec = ag_spec_concat b1.ab_spec b2.ab_spec;
+  ab_impl_type = _;
+  ab_rel = _;
+  ab_parser = impl_zero_copy_array_group_concat length share gather truncate b1.ab_parser v1 b2.ab_parser ();
+}
+
+inline_for_extraction noextract [@@noextract_to "krml"; bundle_get_impl_type_attr]
+let bundle_array_group_choice
+  (#cbor_array_iterator_t: Type)
+  (#cbor_array_iterator_match: perm -> cbor_array_iterator_t -> list cbor -> slprop)
+  (b1: array_bundle cbor_array_iterator_match)
+  (v1: impl_array_group cbor_array_iterator_match b1.ab_typ)
+  (b2: array_bundle cbor_array_iterator_match)
+  (sq: squash (
+    array_group_disjoint b1.ab_typ b2.ab_typ
+  ))
+: Tot (array_bundle cbor_array_iterator_match)
+= {
+  ab_typ = _;
+  ab_spec_type = _;
+  ab_spec = ag_spec_choice b1.ab_spec b2.ab_spec;
+  ab_impl_type = _;
+  ab_rel = _;
+  ab_parser = impl_zero_copy_array_group_choice b1.ab_parser v1 b2.ab_parser;
+}
+
+inline_for_extraction noextract [@@noextract_to "krml"; bundle_get_impl_type_attr]
+let bundle_array_group_zero_or_one
+  (#cbor_array_iterator_t: Type)
+  (#cbor_array_iterator_match: perm -> cbor_array_iterator_t -> list cbor -> slprop)
+  (b1: array_bundle cbor_array_iterator_match)
+  (v1: impl_array_group cbor_array_iterator_match b1.ab_typ)
+  (sq: squash (
+    array_group_is_nonempty b1.ab_typ
+  ))
+: Tot (array_bundle cbor_array_iterator_match)
+= {
+  ab_typ = _;
+  ab_spec_type = _;
+  ab_spec = ag_spec_zero_or_one b1.ab_spec;
+  ab_impl_type = _;
+  ab_rel = _;
+  ab_parser = impl_zero_copy_array_group_zero_or_one b1.ab_parser v1;
+}
+
+inline_for_extraction noextract [@@noextract_to "krml"; bundle_get_impl_type_attr]
+let bundle_array_group_zero_or_more
+  (#cbor_array_iterator_t: Type)
+  (#cbor_array_iterator_match: perm -> cbor_array_iterator_t -> list cbor -> slprop)
+  (share: share_t cbor_array_iterator_match)
+  (gather: gather_t cbor_array_iterator_match)
+  (b1: array_bundle cbor_array_iterator_match)
+  (v1: impl_array_group cbor_array_iterator_match b1.ab_typ)
+  (sq: squash (
+    array_group_concat_unique_strong b1.ab_typ b1.ab_typ /\
+    array_group_is_nonempty b1.ab_typ
+  ))
+: array_bundle cbor_array_iterator_match
+= {
+  ab_typ = _;
+  ab_spec_type = _;
+  ab_spec = ag_spec_zero_or_more b1.ab_spec;
+  ab_impl_type = _;
+  ab_rel = _;
+  ab_parser = impl_zero_copy_array_group_zero_or_more share gather v1 b1.ab_parser ();
+}
+
+inline_for_extraction noextract [@@noextract_to "krml"; bundle_get_impl_type_attr]
+let bundle_array_group_one_or_more
+  (#cbor_array_iterator_t: Type)
+  (#cbor_array_iterator_match: perm -> cbor_array_iterator_t -> list cbor -> slprop)
+  (share: share_t cbor_array_iterator_match)
+  (gather: gather_t cbor_array_iterator_match)
+  (b1: array_bundle cbor_array_iterator_match)
+  (v1: impl_array_group cbor_array_iterator_match b1.ab_typ)
+  (sq: squash (
+    array_group_concat_unique_strong b1.ab_typ b1.ab_typ /\
+    array_group_is_nonempty b1.ab_typ
+  ))
+: array_bundle cbor_array_iterator_match
+= {
+  ab_typ = _;
+  ab_spec_type = _;
+  ab_spec = ag_spec_one_or_more b1.ab_spec;
+  ab_impl_type = _;
+  ab_rel = _;
+  ab_parser = impl_zero_copy_array_group_one_or_more share gather v1 b1.ab_parser ();
+}
