src/cddl/pulse/CDDL.Pulse.Bundle.MapGroup.fst
@@ -1,0 +1,177 @@
+module CDDL.Pulse.Bundle.MapGroup
+include CDDL.Pulse.Bundle.Base
+include CDDL.Pulse.Parse.MapGroup
+open Pulse.Lib.Pervasives
+open CBOR.Spec.API.Type
+open CBOR.Pulse.API.Base
+
+inline_for_extraction noextract [@@noextract_to "krml"]
+noeq
+type map_bundle
+  (#ty: Type0)
+  (vmatch: perm -> ty -> cbor -> slprop)
+= {
+  mb_typ: Ghost.erased (det_map_group);
+  mb_footprint: Ghost.erased typ;
+  mb_footprint_correct: squash (map_group_footprint mb_typ mb_footprint);
+  mb_spec_type: Type0;
+  mb_spec: Ghost.erased (mg_spec mb_typ mb_footprint mb_spec_type true);
+  mb_impl_type: Type0;
+  mb_rel: rel mb_impl_type mb_spec_type;
+  mb_parser: impl_zero_copy_map_group vmatch mb_spec.mg_parser mb_rel;
+}
+
+inline_for_extraction noextract [@@noextract_to "krml"; bundle_get_impl_type_attr ]
+let bundle_map
+  (#ty: Type0)
+  (#vmatch: perm -> ty -> cbor -> slprop)
+  (mb: map_bundle vmatch)
+: Tot (bundle vmatch)
+= {
+  b_typ = _;
+  b_spec_type = _;
+  b_spec = spec_map_group mb.mb_spec;
+  b_impl_type = _;
+  b_rel = _;
+  b_parser = impl_zero_copy_map mb.mb_parser ();
+}
+
+inline_for_extraction noextract [@@noextract_to "krml"; bundle_get_impl_type_attr]
+let bundle_map_ext
+  (#ty: Type0)
+  (#vmatch: perm -> ty -> cbor -> slprop)
+  (mb1: map_bundle vmatch)
+  (#t2: Ghost.erased det_map_group)
+  (#fp2: Ghost.erased typ)
+  (sp2: Ghost.erased (mg_spec t2 fp2 mb1.mb_spec_type true))
+  (sq: squash (
+    impl_zero_copy_map_ext_precond (Ghost.reveal mb1.mb_typ) (mb1.mb_spec.mg_parser) (Ghost.reveal t2) sp2.mg_parser
+  ))
+: Tot (map_bundle vmatch)
+= {
+  mb_typ = _;
+  mb_footprint = _;
+  mb_footprint_correct = ();
+  mb_spec_type = _;
+  mb_spec = sp2;
+  mb_impl_type = _;
+  mb_rel = _;
+  mb_parser = impl_zero_copy_map_ext mb1.mb_parser sp2.mg_parser ()
+}
+
+inline_for_extraction noextract [@@noextract_to "krml"; bundle_get_impl_type_attr]
+let bundle_map_choice
+  (#ty: Type0)
+  (#vmatch: perm -> ty -> cbor -> slprop)
+  (mb1: map_bundle vmatch)
+  (v1: impl_map_group_t vmatch mb1.mb_typ mb1.mb_footprint)
+  (mb2: map_bundle vmatch)
+  (sq: squash (
+    map_group_choice_compatible mb1.mb_typ mb2.mb_typ
+  ))
+: Tot (map_bundle vmatch)
+= {
+  mb_typ = _;
+  mb_footprint = _;
+  mb_footprint_correct = ();
+  mb_spec_type = _;
+  mb_spec = mg_spec_choice mb1.mb_spec mb2.mb_spec;
+  mb_impl_type = _;
+  mb_rel = _;
+  mb_parser = impl_zero_copy_map_choice v1 mb1.mb_parser mb2.mb_parser ();
+}
+
+inline_for_extraction noextract [@@noextract_to "krml"; bundle_get_impl_type_attr]
+let bundle_map_zero_or_one
+  (#ty: Type0)
+  (#vmatch: perm -> ty -> cbor -> slprop)
+  (mb1: map_bundle vmatch)
+  (v1: impl_map_group_t vmatch mb1.mb_typ mb1.mb_footprint)
+  (sq: squash (
+    MapGroupFail? (apply_map_group_det mb1.mb_typ cbor_map_empty)
+  ))
+: Tot (map_bundle vmatch)
+= {
+  mb_typ = _;
+  mb_footprint = _;
+  mb_footprint_correct = ();
+  mb_spec_type = _;
+  mb_spec = mg_spec_zero_or_one mb1.mb_spec;
+  mb_impl_type = _;
+  mb_rel = _;
+  mb_parser = impl_zero_copy_map_zero_or_one v1 mb1.mb_parser ();
+}
+
+inline_for_extraction noextract [@@noextract_to "krml"; bundle_get_impl_type_attr]
+let bundle_map_concat
+  (#ty: Type0)
+  (#vmatch: perm -> ty -> cbor -> slprop)
+  (share: share_t vmatch)
+  (gather: gather_t vmatch)
+  (mb1: map_bundle vmatch)
+  (mb2: map_bundle vmatch)
+  (sq: squash (
+    typ_disjoint mb1.mb_footprint mb2.mb_footprint
+  ))
+: Tot (map_bundle vmatch)
+= {
+  mb_typ = _;
+  mb_footprint = _;
+  mb_footprint_correct = ();
+  mb_spec_type = _;
+  mb_spec = mg_spec_concat mb1.mb_spec mb2.mb_spec;
+  mb_impl_type = _;
+  mb_rel = _;
+  mb_parser = impl_zero_copy_map_concat share gather mb1.mb_parser mb2.mb_parser ();
+}
+
+inline_for_extraction noextract [@@noextract_to "krml"; bundle_get_impl_type_attr]
+let bundle_map_match_item_for
+  (#ty: Type0)
+  (#vmatch: perm -> ty -> cbor -> slprop)
+  (get: map_get_t vmatch)
+  (#key: Ghost.erased cbor)
+  (lkey: with_cbor_literal_t vmatch (Ghost.reveal key))
+  (cut: Ghost.erased bool)
+  (value: bundle vmatch)
+: Tot (map_bundle vmatch)
+= {
+  mb_typ = _;
+  mb_footprint = _;
+  mb_footprint_correct = ();
+  mb_spec_type = _;
+  mb_spec = mg_spec_match_item_for cut key value.b_spec;
+  mb_impl_type = _;
+  mb_rel = _;
+  mb_parser = impl_zero_copy_match_item_for get lkey cut value.b_parser;
+}
+
+module EqTest = CDDL.Spec.EqTest
+
+inline_for_extraction noextract [@@noextract_to "krml"; bundle_get_impl_type_attr]
+let bundle_map_zero_or_more
+  (#ty: Type0)
+  (#vmatch: perm -> ty -> cbor -> slprop)
+  (#cbor_map_iterator_t: Type0)
+  (#cbor_map_iterator_match: perm -> cbor_map_iterator_t -> list (cbor & cbor) -> slprop)
+  (map_iterator_start: map_iterator_start_t vmatch cbor_map_iterator_match)
+  (map_share: share_t cbor_map_iterator_match)
+  (map_gather: gather_t cbor_map_iterator_match)
+  (key: bundle vmatch) // MUST contain function pointers ONLY
+  (key_eq: Ghost.erased (EqTest.eq_test key.b_spec_type))
+  (va1: impl_typ vmatch key.b_typ) // MUST be a function pointer
+  (#key_except: Ghost.erased typ)
+  (va_ex: impl_typ vmatch key_except) // MUST be a function pointer
+  (value: bundle vmatch) // MUST contain function pointers ONLY
+  (va2: impl_typ vmatch value.b_typ) // MUST be a function pointer
+: Tot (map_bundle vmatch)
+= {
+  mb_typ = _;
+  mb_footprint = _;
+  mb_footprint_correct = ();
+  mb_spec_type = _;
+  mb_spec = mg_zero_or_more_match_item key.b_spec key_except value.b_spec;
+  mb_impl_type = _;
+  mb_rel = _;
+  mb_parser = impl_zero_copy_map_zero_or_more map_iterator_start map_share map_gather key_eq key.b_spec va1 key.b_parser va_ex value.b_spec va2 value.b_parser
+}
