src/cddl/pulse/CDDL.Pulse.Bundle.Misc.fst
@@ -1,0 +1,232 @@
+module CDDL.Pulse.Bundle.Misc
+include CDDL.Pulse.Bundle.Base
+include CDDL.Pulse.Parse.Misc
+open Pulse.Lib.Pervasives
+open CBOR.Spec.API.Type
+open CBOR.Pulse.API.Base
+
+inline_for_extraction [@@bundle_get_impl_type_attr]
+let bundle_uint
+  (#cbor_t: Type)
+  (#vmatch: perm -> cbor_t -> cbor -> slprop)
+  (cbor_destr_int64: read_uint64_t vmatch)
+: bundle vmatch
+= {
+  b_typ = _;
+  b_spec_type = _;
+  b_spec = spec_uint;
+  b_impl_type = _;
+  b_rel = _;
+  b_parser = impl_copyful_pure_as_zero_copy (impl_copyful_uint cbor_destr_int64);
+}
+
+inline_for_extraction [@@bundle_get_impl_type_attr]
+let bundle_nint
+  (#cbor_t: Type)
+  (#vmatch: perm -> cbor_t -> cbor -> slprop)
+  (cbor_destr_int64: read_uint64_t vmatch)
+: bundle vmatch
+= {
+  b_typ = _;
+  b_spec_type = _;
+  b_spec = spec_nint;
+  b_impl_type = _;
+  b_rel = _;
+  b_parser = impl_copyful_pure_as_zero_copy (impl_copyful_nint cbor_destr_int64);
+}
+
+module U64 = FStar.UInt64
+
+inline_for_extraction [@@bundle_get_impl_type_attr]
+let bundle_int_range_uint64
+  (#cbor_t: Type)
+  (#vmatch: perm -> cbor_t -> cbor -> slprop)
+  (cbor_destr_int64: read_uint64_t vmatch)
+  (lo hi: Ghost.erased U64.t)
+: bundle vmatch
+= {
+  b_typ = _;
+  b_spec_type = _;
+  b_spec = spec_int_range_uint64 lo hi;
+  b_impl_type = _;
+  b_rel = _;
+  b_parser = impl_copyful_pure_as_zero_copy (impl_copyful_int_range_uint64 cbor_destr_int64 lo hi);
+}
+
+module I64 = FStar.Int64
+
+inline_for_extraction [@@bundle_get_impl_type_attr]
+let bundle_int_range_int64
+  (#cbor_t: Type)
+  (#vmatch: perm -> cbor_t -> cbor -> slprop)
+  (cbor_get_major_type: get_major_type_t vmatch)
+  (cbor_destr_int64: read_uint64_t vmatch)
+  (lo hi: Ghost.erased I64.t)
+: bundle vmatch
+= {
+  b_typ = _;
+  b_spec_type = _;
+  b_spec = spec_int_range_int64 lo hi;
+  b_impl_type = _;
+  b_rel = _;
+  b_parser = impl_copyful_pure_as_zero_copy (impl_copyful_int_range_int64 cbor_get_major_type cbor_destr_int64 lo hi);
+}
+
+inline_for_extraction [@@bundle_get_impl_type_attr]
+let bundle_int_range_neg_int64
+  (#cbor_t: Type)
+  (#vmatch: perm -> cbor_t -> cbor -> slprop)
+  (cbor_destr_int64: read_uint64_t vmatch)
+  (lo hi: Ghost.erased U64.t)
+: bundle vmatch
+= {
+  b_typ = _;
+  b_spec_type = _;
+  b_spec = spec_int_range_neg_int64 lo hi;
+  b_impl_type = _;
+  b_rel = _;
+  b_parser = impl_copyful_pure_as_zero_copy (impl_copyful_int_range_neg_int64 cbor_destr_int64 lo hi);
+}
+
+inline_for_extraction [@@bundle_get_impl_type_attr]
+let bundle_bytes
+  (#cbor_t: Type)
+  (#vmatch: perm -> cbor_t -> cbor -> slprop)
+  (cbor_destr_string: get_string_t vmatch)
+: bundle vmatch
+= {
+  b_typ = _;
+  b_spec_type = _;
+  b_spec = spec_bstr;
+  b_impl_type = _;
+  b_rel = _;
+  b_parser = impl_zero_copy_bytes cbor_destr_string;
+}
+
+inline_for_extraction [@@bundle_get_impl_type_attr]
+let bundle_text
+  (#cbor_t: Type)
+  (#vmatch: perm -> cbor_t -> cbor -> slprop)
+  (cbor_destr_string: get_string_t vmatch)
+: bundle vmatch
+= {
+  b_typ = _;
+  b_spec_type = _;
+  b_spec = spec_tstr;
+  b_impl_type = _;
+  b_rel = _;
+  b_parser = impl_zero_copy_text cbor_destr_string;
+}
+
+inline_for_extraction [@@bundle_get_impl_type_attr]
+let bundle_str_size
+  (#cbor_t: Type)
+  (#vmatch: perm -> cbor_t -> cbor -> slprop)
+  (cbor_destr_string: get_string_t vmatch)
+  (mt: Ghost.erased major_type_byte_string_or_text_string)
+  (lo hi: Ghost.erased U64.t)
+: bundle vmatch
+= {
+  b_typ = _;
+  b_spec_type = _;
+  b_spec = (spec_str_size mt lo hi);
+  b_impl_type = _;
+  b_rel = _;
+  b_parser = impl_zero_copy_str_size cbor_destr_string mt lo hi;
+}
+
+inline_for_extraction [@@bundle_get_impl_type_attr]
+let bundle_simple
+  (#cbor_t: Type)
+  (#vmatch: perm -> cbor_t -> cbor -> slprop)
+  (cbor_destr_simple: read_simple_value_t vmatch)
+: bundle vmatch
+= {
+  b_typ = _;
+  b_spec_type = _;
+  b_spec = spec_simple;
+  b_impl_type = _;
+  b_rel = _;
+  b_parser = impl_copyful_pure_as_zero_copy (impl_copyful_simple cbor_destr_simple);
+}
+
+inline_for_extraction [@@bundle_get_impl_type_attr]
+let bundle_bool
+  (#cbor_t: Type)
+  (#vmatch: perm -> cbor_t -> cbor -> slprop)
+  (cbor_destr_simple: read_simple_value_t vmatch)
+: bundle vmatch
+= {
+  b_typ = _;
+  b_spec_type = _;
+  b_spec = spec_bool;
+  b_impl_type = _;
+  b_rel = _;
+  b_parser = impl_copyful_pure_as_zero_copy (impl_copyful_bool cbor_destr_simple);
+}
+
+inline_for_extraction [@@bundle_get_impl_type_attr]
+let bundle_tagged_some
+  (#cbor_t: Type)
+  (#vmatch: perm -> cbor_t -> cbor -> slprop)
+  (cbor_get_tagged_payload: get_tagged_payload_t vmatch)
+  (tag: Ghost.erased U64.t)
+  (b: bundle vmatch)
+: bundle vmatch
+= {
+  b_typ = _;
+  b_spec_type = _;
+  b_spec = spec_tag_some tag b.b_spec;
+  b_impl_type = _;
+  b_rel = _;
+  b_parser = impl_zero_copy_tagged_some cbor_get_tagged_payload tag b.b_parser;
+}
+
+inline_for_extraction [@@bundle_get_impl_type_attr]
+let bundle_tagged_none
+  (#cbor_t: Type)
+  (#vmatch: perm -> cbor_t -> cbor -> slprop)
+  (cbor_get_tagged_tag: get_tagged_tag_t vmatch)
+  (cbor_get_tagged_payload: get_tagged_payload_t vmatch)
+  (b: bundle vmatch)
+: bundle vmatch
+= {
+  b_typ = _;
+  b_spec_type = _;
+  b_spec = spec_tag_none b.b_spec;
+  b_impl_type = _;
+  b_rel = _;
+  b_parser = impl_zero_copy_tagged_none cbor_get_tagged_tag cbor_get_tagged_payload b.b_parser;
+}
+
+inline_for_extraction [@@bundle_get_impl_type_attr]
+let bundle_det_cbor
+  (#cbor_t: Type)
+  (#vmatch: perm -> cbor_t -> cbor -> slprop)
+  (#vmatch': perm -> cbor_t -> cbor -> slprop)
+  (cbor_destr_string: get_string_t vmatch)
+  (cbor_det_parse: cbor_det_parse_t vmatch')
+  (b: bundle vmatch')
+: bundle vmatch
+= {
+  b_typ = _;
+  b_spec_type = _;
+  b_spec = spec_bstr_cbor_det b.b_spec;
+  b_impl_type = _;
+  b_rel = _;
+  b_parser = impl_zero_copy_det_cbor cbor_destr_string cbor_det_parse b.b_spec b.b_parser;
+}
+
+inline_for_extraction [@@bundle_get_impl_type_attr]
+let bundle_any
+  (#cbor_t: Type)
+  (vmatch: perm -> cbor_t -> cbor -> slprop)
+: bundle vmatch
+= {
+  b_typ = _;
+  b_spec_type = _;
+  b_spec = spec_any;
+  b_impl_type = _;
+  b_rel = _;
+  b_parser = impl_zero_copy_any vmatch;
+}
